CollapsingTowers/TwoLevelMut/LogicalEquiv/LogicalRelation.lean
@@ -4,8 +4,13 @@ import CollapsingTowers.TwoLevelMut.LogicalEquiv.World
 -- (σ₀, σ₁) : 𝓦 ≜ ∀ 𝓦(l₀, l₁). σ₀(l₁) = σ₀(l₁)
 @[simp]
 def log_equiv_store (𝓦 : World) (σ₀ σ₁ : Store) : Prop :=
-  ∀ l₀ l₁, 𝓦 l₀ l₁ →
-  ∃ n, binds l₀ (.lit n) σ₀ ∧ binds l₁ (.lit n) σ₁
+  bijection 𝓦 ∧ (
+  ∀ l₀ l₁,
+    𝓦 l₀ l₁ →
+    ∃ n,
+      binds l₀ (.lit n) σ₀ ∧
+      binds l₁ (.lit n) σ₁
+  )
 
 mutual
 @[simp]
@@ -41,10 +46,10 @@ def log_equiv_value : World → Expr → Expr → Ty → Prop
 --   (𝓦₀, e₀, e₁) |
 --   ∀ (σ₀, σ₁) : 𝓦₀.
 --   ∃ ω₀, ω₁, v₀, v₁, (𝓦₁ ⊒ 𝓦₀).
---   ⟨σ₀, e₀⟩ ⇝* ⟨ω₀, v₀⟩ ∧
---   ⟨σ₁, e₁⟩ ⇝* ⟨ω₁, v₁⟩ ∧
---   (ω₀, ω₁) : 𝓦₁ ∧
---   (𝓦₁, v₀, v₁) ∈ 𝓥⟦τ⟧
+--     ⟨σ₀, e₀⟩ ⇝* ⟨ω₀, v₀⟩ ∧
+--     ⟨σ₁, e₁⟩ ⇝* ⟨ω₁, v₁⟩ ∧
+--     (ω₀, ω₁) : 𝓦₁ ∧
+--     (𝓦₁, v₀, v₁) ∈ 𝓥⟦τ⟧
 -- }
 @[simp]
 def log_equiv_expr (𝓦₀ : World) (e₀ e₁ : Expr) (τ : Ty) : Prop :=
@@ -76,3 +81,63 @@ def log_equiv (Γ : TEnv) (e₀ e₁ : Expr) (τ : Ty) : Prop :=
   ∀ 𝓦 γ₀ γ₁,
     log_equiv_env 𝓦 γ₀ γ₁ Γ →
     log_equiv_expr 𝓦 (msubst γ₀ e₀) (msubst γ₁ e₁) τ
+
+lemma log_equiv_value.antimono :
+  ∀ 𝓦₀ 𝓦₁ v₀ v₁ τ,
+    log_equiv_value 𝓦₀ v₀ v₁ τ →
+    (𝓦₁ ⊒ 𝓦₀) →
+    log_equiv_value 𝓦₁ v₀ v₁ τ :=
+  by
+  intros 𝓦₀ 𝓦₁ v₀ v₁ τ Hsem_value Hfuture₀
+  cases τ
+  case nat =>
+    cases v₀ <;> try simp at Hsem_value
+    case lit n₀ =>
+    cases v₁ <;> try simp at Hsem_value
+    case lit n₁ =>
+    simp; apply Hsem_value
+  case arrow τ𝕒 τ𝕓 φ =>
+    cases v₀ <;> try simp at Hsem_value
+    case lam e₀ =>
+    cases v₁ <;> try simp at Hsem_value
+    case lam e₁ =>
+    cases φ <;> simp only [log_equiv_value] at Hsem_value <;> try contradiction
+    have ⟨Hwf₀, HG₀, Hwf₁, HG₁, Hsem_value⟩ := Hsem_value
+    simp only [log_equiv_value]
+    constructor; apply Hwf₀
+    constructor; apply HG₀
+    constructor; apply Hwf₁
+    constructor; apply HG₁
+    intros 𝓦₂ v₀ v₁ Hfuture₁
+    apply Hsem_value
+    apply World.future.trans _ _ _ Hfuture₁ Hfuture₀
+  case unit =>
+    cases v₀ <;> try simp at Hsem_value
+    case unit =>
+    cases v₁ <;> try simp at Hsem_value
+    case unit =>
+    simp
+  case ref τ =>
+    cases v₀ <;> try simp at Hsem_value
+    case loc l₀ =>
+    cases v₁ <;> try simp at Hsem_value
+    case loc l₁ =>
+    cases τ <;> simp only [log_equiv_value] at Hsem_value <;> try contradiction
+    simp only [log_equiv_value]
+    apply Hfuture₀; apply Hsem_value
+  case fragment => simp at Hsem_value
+  case rep => simp at Hsem_value
+
+lemma log_equiv_env.antimono :
+  ∀ 𝓦₀ 𝓦₁ γ₀ γ₁ Γ,
+    log_equiv_env 𝓦₀ γ₀ γ₁ Γ →
+    (𝓦₁ ⊒ 𝓦₀) →
+    log_equiv_env 𝓦₁ γ₀ γ₁ Γ :=
+  by
+  intros 𝓦₀ 𝓦₁ γ₀ γ₁ Γ HsemΓ Hfuture₀
+  induction HsemΓ
+  case nil => apply log_equiv_env.nil
+  case cons Hsem_value _ IH =>
+    apply log_equiv_env.cons
+    apply log_equiv_value.antimono; apply Hsem_value; apply Hfuture₀
+    apply IH
